changed formalisation of commitment scheme

NSNM_Definition.ec
@@ -31,7 +31,7 @@ module type AdvSNM = {
 
 
 module type Simulator = {
-  proc simulate(pk : value, r : snm_relation, dd : message distr) : message *  commitment * openingkey
+  proc simulate(pk : value, r : snm_relation, dd : message distr) : message 
 }.
 
 
@@ -52,11 +52,11 @@ module SG0(A : AdvSNM) = {
 
 module SG1(A : AdvSNM, S : Simulator) = {
   proc main(h : advice) : bool = {
-    var pk, m, c', d', m', md, mrel;    
+    var pk, m, m', md, mrel;    
     pk                 <$ Dpk; 
     (md, mrel)         <- A.init(pk,h);
     m                  <$ md;
-    (m', c',  d')      <- S.simulate(pk, mrel, md);
+    m'                 <- S.simulate(pk, mrel, md);
     return mrel m m';
   }
 }.
@@ -92,11 +92,11 @@ module SEG0(CS:CommitmentScheme, A : AdvSNM) = {
 
 module SEG1(CS:CommitmentScheme, A : AdvSNM, S : Simulator) = {
   proc main(h : advice) : bool = {
-    var m,m',pk,c,d, ssnmdistr, rel;    
+    var m,m',pk, ssnmdistr, rel;    
     pk                 <- CS.gen(); 
     (ssnmdistr, rel)   <- A.init(pk, h);
     m                  <$ ssnmdistr;
-    (m',c,d)           <- S.simulate(pk, rel, ssnmdistr);
+    m'           <- S.simulate(pk, rel, ssnmdistr);
     return rel m m';
   }
 }.
