Binding_adv_wrapper.ec
@@ -60,7 +60,7 @@ qed.
 local lemma final &m h :  forall (S <: Simulator {A', B, A}),
   Pr[ BindingExperiment(A'(A)).main() @ &m : res ] <= 
   2%r * (Pr[ SG0(B(A'(A))).main(h) @ &m : res ] - Pr[ SG1(B(A'(A)),S).main(h) @ &m : res ]) 
-   + 6%r * Pr[ UnpredGame(BG(A'(A))).main() @ &m : res ].
+   + 6%r * Pr[ UnpredGame(BU(A'(A))).main() @ &m : res ].
 proof.
 move => S.  
 apply (nsnm_pure_binding (A'(A)) Ag_ll ba' &m h S ). 
@@ -70,13 +70,13 @@ qed.
 lemma nsnm_pure_binding_2 &m h :  forall (S <: Simulator {A', B, A}),
   Pr[ BindingExperiment(A).main() @ &m : res ] <= 
   2%r * (Pr[ SG0(B(A'(A))).main(h) @ &m : res ] - Pr[ SG1(B(A'(A)),S).main(h) @ &m : res ]) 
-   + 6%r * Pr[ UnpredGame(BG(A'(A))).main() @ &m : res ].
+   + 6%r * Pr[ UnpredGame(BU(A'(A))).main() @ &m : res ].
 proof.
 move => S. 
 have : Pr[ BindingExperiment(A).main() @ &m : res ] <= Pr[ BindingExperiment(A'(A)).main() @ &m : res ]. apply l1. progress.  
 have : Pr[ BindingExperiment(A'(A)).main() @ &m : res ] <= 
   2%r * (Pr[ SG0(B(A'(A))).main(h) @ &m : res ] - Pr[ SG1(B(A'(A)),S).main(h) @ &m : res ]) 
-   + 6%r * Pr[ UnpredGame(BG(A'(A))).main() @ &m : res ].
+   + 6%r * Pr[ UnpredGame(BU(A'(A))).main() @ &m : res ].
 apply (final &m h S). progress.
 smt. 
 qed.
